Starting ACCSExamples

theories/Labelled_Transition_System/Examples_of_LTS/VACCS/VACCS_Instance.v
@@ -1524,6 +1524,162 @@ Proof.
       { eapply Hp. simpl. lia. } inversion eq1. inversion eq2. eauto.
 Qed.
 
+(* Scheme proc_gproc_ind := Induction for proc Sort Prop
+  with gproc_proc_ind := Induction for gproc Sort Prop.
+
+
+Definition PPS (P : proc -> Prop) (p : gproc) := P (g p).
+
+Lemma proc_gproc_myinduction : ∀ (P : proc → Prop),
+         (∀ p : proc, P p → ∀ p0 : proc, P p0 → P (p ‖ p0))
+         → (∀ n : nat, P n)
+           → (∀ (n : nat) (p : proc), P p → P (rec n • p))
+             → (∀ (e : Equation Data) (p : proc), P p → ∀ p0 : proc, P p0 → P (If e
+                                                                                Then p
+                                                                                Else p0))
+               → (∀ (c : Channel) (d : Data), P (c ! d • 𝟘))
+                 → (∀ g0 : gproc, P (g g0) → P g0)
+                   → P (g ①)
+                     → P (g 𝟘)
+                       → (∀ (c : Channel) (p : proc), P p → P (g (gpr_input c p)))
+                         → (∀ p : proc, P p → P (g (t • p)))
+                           → (∀ g1 : gproc, P (g g1) → ∀ g0 : gproc, P (g g0) → P (g (g1 + g0))) → ∀ p : proc, P p.
+Proof.
+
+intros. revert p. eapply proc_gproc_ind.
+- eauto.
+- eauto.
+- eauto.
+- eauto.
+- eauto.
+- intros. instantiate (1 := PPS P) in H10. unfold PPS in H10. eauto.
+- intros. unfold PPS. eauto.
+- intros. unfold PPS. eauto.
+- intros. unfold PPS. eauto.
+- intros. unfold PPS. eauto.
+- intros. unfold PPS. eauto.
+Qed.
+
+(*Definition cgr_subst2 p := forall q q' x, q ≡* q' → pr_subst x p q ≡* pr_subst x p q'. *)
+
+(* Substition lemma, needed to contextualise the equivalence *)
+Lemma cgr_subst1 p q q' x : q ≡* q' → pr_subst x p q ≡* pr_subst x p q'.
+Proof.
+revert q q' x.
+
+(*
+(* Version with the induction principle with the same P for proc and gproc *)
+induction p,(size3) using proc_gproc_myinduction; intros; simpl.
+(* have to specify P0 with functional induction (size3 p) *)
+
+- apply cgr_fullpar.
+    apply IHn. assumption.
+    apply IHn0. assumption.
+- destruct (decide (x = _x)). assumption. reflexivity.
+- apply cgr_full_if.
+    apply IHn. assumption.
+    apply IHn0. assumption.
+- destruct (decide (x0 = x)).
+    * reflexivity.
+    * apply cgr_recursion. eapply IHn. assumption.
+- eauto with cgr.
+- eauto.
+- reflexivity.
+- reflexivity.
+- apply cgr_input. eapply IHn. apply NewVar_Respects_Congruence. assumption.
+- apply cgr_tau. eapply IHn. assumption.
+- apply cgr_fullchoice.
+  * eapply IHn. assumption.
+  * eapply IHn0. assumption. *)
+
+
+(* Version with the induction principle (not with dependent *)
+(*
+functional induction (size3 p) using size3_ind; intros; simpl; auto.
+
+- apply cgr_fullpar.
+    apply IHn. assumption.
+    apply IHn0. assumption.
+- destruct (decide (x = _x)). assumption. reflexivity.
+- apply cgr_full_if.
+    apply IHn. assumption.
+    apply IHn0. assumption.
+- destruct (decide (x0 = x)).
+    * reflexivity.
+    * apply cgr_recursion. eapply IHn. assumption.
+- eauto with cgr.
+- (* cant move forward due to dependent inductive types *)
+*)
+
+
+(* Version with the mutual induction principle *)
+(*
+einduction p using proc_gproc_ind; simpl;  intros.
+
+- apply cgr_fullpar.
+    apply IHp0_1. assumption.
+    apply IHp0_2. assumption.
+- destruct (decide (x = n)). assumption. reflexivity.
+- destruct (decide (x = n)). reflexivity. apply cgr_recursion. apply IHp0. assumption.
+- apply cgr_full_if.
+    apply IHp0_1. assumption.
+    apply IHp0_2. assumption.
+- eauto with cgr.
+- instantiate (1 := cgr_subst2) in IHp0.
+  unfold cgr_subst2 in IHp0. apply IHp0. assumption.
+- unfold cgr_subst2. simpl; intros. auto with cgr.
+- unfold cgr_subst2. simpl; intros. auto with cgr.
+- unfold cgr_subst2. simpl; intros. apply cgr_input. apply IHp0. apply NewVar_Respects_Congruence. assumption.
+- unfold cgr_subst2. simpl; intros. apply cgr_tau. apply IHp0. assumption.
+- unfold cgr_subst2. simpl; intros. apply cgr_fullchoice.
+  * unfold cgr_subst2 in IHp0. apply IHp0. assumption.
+  * unfold cgr_subst2 in IHp1. apply IHp1. assumption. *)
+
+einduction p using proc_gproc_myinduction; simpl;  intros.
+
+- apply cgr_fullpar.
+    apply IHp0_1. assumption.
+    apply IHp0_2. assumption.
+- destruct (decide (x = n)). assumption. reflexivity.
+- destruct (decide (x = n)). reflexivity. apply cgr_recursion. apply IHp0. assumption.
+- apply cgr_full_if.
+    apply IHp0_1. assumption.
+    apply IHp0_2. assumption.
+- eauto with cgr.
+- apply IHp0. assumption.
+- reflexivity.
+- reflexivity.
+- apply cgr_input. apply IHp0. apply NewVar_Respects_Congruence. assumption.
+- apply cgr_tau. apply IHp0. assumption.
+- apply cgr_fullchoice.
+  * apply IHp0. assumption.
+  * apply IHp1. assumption.
+
+(*  (* Old version *)
+(* Induction on the size of p*)
+induction p as (p & Hp) using
+    (well_founded_induction (wf_inverse_image _ nat _ size Nat.lt_wf_0)).
+destruct p; intros; simpl.
+  - apply cgr_fullpar.
+    apply Hp. simpl. auto with arith. assumption.
+    apply Hp. simpl. auto with arith. assumption.
+  - destruct (decide (x = n)). assumption. reflexivity.
+  - destruct (decide (x = n)). reflexivity. apply cgr_recursion. apply Hp. simpl. auto. assumption.
+  - apply cgr_full_if.
+    apply Hp. simpl. auto with arith. assumption.
+    apply Hp. simpl. auto with arith. assumption.
+  - eauto with cgr.
+  - destruct g0; simpl.
+    * reflexivity.
+    * reflexivity.
+    * apply cgr_input. apply Hp. simpl. auto with arith. apply NewVar_Respects_Congruence. assumption.
+    * apply cgr_tau. apply Hp. simpl. auto with arith. assumption.
+    * apply cgr_fullchoice.
+      assert (pr_subst x (g g0_1) q ≡* pr_subst x (g g0_1) q'). apply Hp. simpl. auto with arith. assumption.
+      auto. assert (pr_subst x (g g0_2) q ≡* pr_subst x (g g0_2) q'). apply Hp. simpl. auto with arith. assumption.
+      auto. *)
+Qed. *)
+
 (* ≡ respects the substitution (in recursion) of his variable *)
 Lemma cgr_step_subst2 : forall p p' q x, p ≡ p' → pr_subst x p q ≡ pr_subst x p' q.
 Proof.
